Some cleanups, and some work on the alphabetised lattice.

theories/alpha/utp_alpha_lattice.thy
@@ -42,11 +42,17 @@ end
 definition BotA :: "'VALUE ALPHABET \<Rightarrow> 'VALUE WF_ALPHA_PREDICATE" ("\<bottom>\<^bsub>_\<^esub>") where
 "BotA = TrueA"
 
+theorem BotA_rep_eq:
+  "Rep_WF_ALPHA_PREDICATE \<bottom>\<^bsub>a \<^esub>= (a, bot)"
+  by (simp add:BotA_def TrueA_rep_eq bot_WF_PREDICATE_def)
+
 definition TopA :: "'VALUE ALPHABET \<Rightarrow> 'VALUE WF_ALPHA_PREDICATE" ("\<top>\<^bsub>_\<^esub>") where
 "TopA = FalseA"
 
-declare sup_WF_ALPHA_PREDICATE_def [evala]
-declare inf_WF_ALPHA_PREDICATE_def [evala]
+theorem TopA_rep_eq:
+  "Rep_WF_ALPHA_PREDICATE \<top>\<^bsub>a \<^esub>= (a, top)"
+  by (simp add:TopA_def FalseA_rep_eq top_WF_PREDICATE_def)
+
 declare BotA_def [evala]
 declare TopA_def [evala]
 
@@ -56,56 +62,123 @@ lemma RefinementA_intro [intro]:
   apply (simp add:EvalA_def)
 done
 
-definition SupP ::
+definition SupA ::
   "'VALUE ALPHABET \<Rightarrow>
    'VALUE WF_ALPHA_PREDICATE set \<Rightarrow>
    'VALUE WF_ALPHA_PREDICATE" where
 "\<forall> p\<in>ps. \<alpha> p \<subseteq>\<^sub>f a \<Longrightarrow>
- SupP a ps =
+ SupA a ps =
  (if ps = {} then \<bottom>\<^bsub>a\<^esub> else
    Abs_WF_ALPHA_PREDICATE (a, \<Squnion> (\<pi> ` ps)))"
 
-definition InfP ::
+theorem SupA_rep_eq:
+  "\<forall> p\<in>ps. \<alpha> p \<subseteq>\<^sub>f a \<Longrightarrow>
+   Rep_WF_ALPHA_PREDICATE (SupA a ps) = (a, \<Squnion> (\<pi> ` ps))"
+  apply (subgoal_tac "(a, \<Squnion> (\<pi> ` ps)) \<in> WF_ALPHA_PREDICATE")
+  apply (simp add:SupA_def BotA_rep_eq)
+  apply (simp add:WF_ALPHA_PREDICATE_def WF_PREDICATE_OVER_def)
+  apply (auto intro:unrest)
+done
+
+definition InfA ::
   "'VALUE ALPHABET \<Rightarrow>
    'VALUE WF_ALPHA_PREDICATE set \<Rightarrow>
    'VALUE WF_ALPHA_PREDICATE" where
 "\<forall> p\<in>ps. \<alpha> p \<subseteq>\<^sub>f a \<Longrightarrow>
- InfP a ps =
+ InfA a ps =
  (if ps = {} then \<top>\<^bsub>a\<^esub> else
    Abs_WF_ALPHA_PREDICATE (a, \<Sqinter> (\<pi> ` ps)))"
 
-(*
-lemma InfP_alphabet:
-  "\<forall> p\<in>ps. \<alpha> p \<subseteq>\<^sub>f a \<Longrightarrow> \<alpha> (InfP a ps) = a"
-  apply (simp add:InfP_def)
-  apply (utp_alpha_tac)
+theorem InfA_rep_eq:
+  "\<forall> p\<in>ps. \<alpha> p \<subseteq>\<^sub>f a \<Longrightarrow>
+   Rep_WF_ALPHA_PREDICATE (InfA a ps) = (a, \<Sqinter> (\<pi> ` ps))"
+  apply (subgoal_tac "(a, \<Sqinter> (\<pi> ` ps)) \<in> WF_ALPHA_PREDICATE")
+  apply (simp add:InfA_def TopA_rep_eq)
+  apply (simp add:WF_ALPHA_PREDICATE_def WF_PREDICATE_OVER_def)
+  apply (auto intro:unrest)
+done
 
-lemma "\<alpha> P = a \<Longrightarrow> P \<sqsubseteq> InfP a S"
+subsection {* Alphabet theorems *} 
+
+lemma TopA_alphabet [alphabet]:
+  "\<alpha> \<top>\<^bsub>a\<^esub> = a"
+  by (simp add:pred_alphabet_def TopA_rep_eq)
+
+lemma BotA_alphabet [alphabet]:
+  "\<alpha> \<bottom>\<^bsub>a\<^esub> = a"
+  by (simp add:pred_alphabet_def BotA_rep_eq)
+
+lemma sup_alphabet [alphabet]:
+  "\<alpha> (p \<squnion> q) = \<alpha> p \<union>\<^sub>f \<alpha> q"
+  by (simp add:sup_WF_ALPHA_PREDICATE_def alphabet)
+
+lemma inf_alphabet [alphabet]:
+  "\<alpha> (p \<sqinter> q) = \<alpha> p \<union>\<^sub>f \<alpha> q"
+  by (simp add:inf_WF_ALPHA_PREDICATE_def alphabet)
+
+lemma SupA_alphabet [alphabet]:
+  "\<forall> p\<in>ps. \<alpha> p \<subseteq>\<^sub>f a \<Longrightarrow> \<alpha> (SupA a ps) = a"
+  by (simp add:pred_alphabet_def SupA_rep_eq)
+
+lemma InfA_alphabet [alphabet]:
+  "\<forall> p\<in>ps. \<alpha> p \<subseteq>\<^sub>f a \<Longrightarrow> \<alpha> (InfA a ps) = a"
+  by (simp add:pred_alphabet_def InfA_rep_eq)
+
+subsubsection {* Evaluation laws *}
+
+lemma EvalA_sup [evala]:
+  "\<lbrakk>p \<squnion> q\<rbrakk>\<pi> = \<lbrakk>p\<rbrakk>\<pi> \<squnion> \<lbrakk>q\<rbrakk>\<pi>"
+  by (simp add: sup_WF_ALPHA_PREDICATE_def sup_WF_PREDICATE_def evala)
+
+lemma EvalA_inf [evala]:
+  "\<lbrakk>p \<sqinter> q\<rbrakk>\<pi> = \<lbrakk>p\<rbrakk>\<pi> \<sqinter> \<lbrakk>q\<rbrakk>\<pi>"
+  by (simp add: inf_WF_ALPHA_PREDICATE_def inf_WF_PREDICATE_def evala)
+  
+lemma EvalA_SupA [evala]: 
+  "\<lbrakk>\<forall> p\<in>ps. \<alpha> p \<subseteq>\<^sub>f a \<rbrakk> \<Longrightarrow> \<lbrakk>SupA a ps\<rbrakk>\<pi> = \<Squnion> (EvalA ` ps)"
+  by (simp add:SupA_rep_eq EvalA_def image_def)
+
+lemma EvalA_InfA [evala]: 
+  "\<lbrakk>\<forall> p\<in>ps. \<alpha> p \<subseteq>\<^sub>f a \<rbrakk> \<Longrightarrow> \<lbrakk>InfA a ps\<rbrakk>\<pi> = \<Sqinter> (EvalA ` ps)"
+  by (simp add:InfA_rep_eq EvalA_def image_def)
+
+  
+lemma L1: 
+  "\<lbrakk> \<alpha> P = a; \<forall> p\<in>S. \<alpha> p = a \<rbrakk> \<Longrightarrow>
+   P \<sqsubseteq> InfA a S \<longleftrightarrow> (\<forall> X\<in>S. P \<sqsubseteq> X)"
+  by (simp add:EvalA_RefinementA alphabet evala Lattice_L1)
+
+lemma L2:
+  "\<lbrakk> \<alpha> Q = a; \<forall> p\<in>S. \<alpha> p = a \<rbrakk> \<Longrightarrow>
+  ((SupA a S) \<sqinter> Q) = SupA a {P \<sqinter> Q | P. P \<in> S}"
+  apply (subgoal_tac "\<forall> p \<in> {P \<sqinter> Q | P. P \<in> S}. \<alpha> p = a")
+  apply (rule EvalA_intro)
+  apply (simp add:alphabet)
+  apply (simp add:EvalA_SupA EvalA_inf Lattice_L2)
+  apply (subgoal_tac "{P \<sqinter> \<lbrakk>Q\<rbrakk>\<pi> |P. P \<in> EvalA ` S} = EvalA ` {P \<sqinter> Q |P. P \<in> S}")
+  apply (simp)
+oops
 
 subsection {* Fixed Points *}
 
 definition WFP ::
   "'VALUE ALPHABET \<Rightarrow>
    'VALUE ALPHA_FUNCTION \<Rightarrow>
-   'VALUE ALPHA_PREDICATE" ("\<mu>") where
-"a \<in> WF_ALPHABET \<and>
- f \<in> WF_ALPHA_FUNCTION_BETWEEN a a \<longrightarrow>
- WFP a f = \<Squnion> a {x \<in> WF_ALPHA_PREDICATE_OVER a . f x \<sqsubseteq> x}"
+   'VALUE WF_ALPHA_PREDICATE" where
+"f \<in> WF_ALPHA_FUNCTION_BETWEEN a a \<longrightarrow>
+ WFP a f = SupA a {x \<in> WF_ALPHA_PREDICATE_OVER a . f x \<le> x}"
 
 definition SFP ::
-  "'TYPE ALPHABET \<Rightarrow>
-   ('VALUE, 'TYPE) ALPHA_FUNCTION \<Rightarrow>
-   ('VALUE, 'TYPE) ALPHA_PREDICATE" ("\<nu>") where
-"a \<in> WF_ALPHABET \<and>
- f \<in> WF_ALPHA_FUNCTION_BETWEEN a a \<longrightarrow>
- SFP a f = \<Sqinter> a {x \<in> WF_ALPHA_PREDICATE_OVER a . x \<sqsubseteq> f x}"
-
+  "'VALUE ALPHABET \<Rightarrow>
+   'VALUE ALPHA_FUNCTION \<Rightarrow>
+   'VALUE WF_ALPHA_PREDICATE" where
+"f \<in> WF_ALPHA_FUNCTION_BETWEEN a a \<longrightarrow>
+ SFP a f = InfA a {x \<in> WF_ALPHA_PREDICATE_OVER a . x \<le> f x}"
 
 lemma BotA_least: "\<bottom>\<^bsub>\<alpha> p\<^esub> \<sqsubseteq> p"
   by (utp_alpha_tac, utp_pred_tac)
 
 lemma TopA_greatest: "p \<sqsubseteq> \<top>\<^bsub>\<alpha> p\<^esub>"
   by (utp_alpha_tac, utp_pred_tac)
-*)
 
 end
