theories/tactics/utp_alpha_tac.thy
@@ -153,6 +153,9 @@ declare ContradictionA_def [evala]
 declare less_eq_WF_ALPHA_PREDICATE_def [evala]
 declare less_WF_ALPHA_PREDICATE_def [evala]
 
+lemma EvalA_RefinementA: "p \<sqsubseteq> q \<longleftrightarrow> \<alpha> p = \<alpha> q \<and> \<lbrakk>p\<rbrakk>\<pi> \<sqsubseteq> \<lbrakk>q\<rbrakk>\<pi>"
+  by (simp add:less_eq_WF_ALPHA_PREDICATE_def less_eq_WF_PREDICATE_def evala eval alphabet)
+
 subsection {* Proof Tactics *}
 
 text {*
